\section{Fresnel Reflectivity Derivation}
%========================================
\label{sec:fresnel_equations}
This section merely derives the Fresnel reflectivity equations used in the CRTM microwave sea surface emissivity from the more typical equations.

As defined in section 1.5.2 in \citet{BornWolf_1999}, the complex amplitudes of the reflected waves parallel (vertical) and perpendicular (horizontal) to the plane of incidence of an air/ocean water interface are given by,
\begin{equation}
  R_{\parallel} = \frac{n_{2}\cos\theta_{i} - n_{1}\cos\theta_{t}}{n_{2}\cos\theta_{i} + n_{1}\cos\theta_{t}}.A_{\parallel}
  \label{eqn:Rv_amplitude}
\end{equation}
and
\begin{equation}
  R_{\perp} = \frac{n_{1}\cos\theta_{i} - n_{2}\cos\theta_{t}}{n_{1}\cos\theta_{i} + n_{2}\cos\theta_{t}}.A_{\perp}
  \label{eqn:Rh_amplitude}
\end{equation}
where $n_{1}$ and $n_{2}$ are the refractive indices of air and ocean water respectively, $\theta_{i}$ and $\theta_{t}$ the angles of incidence and transmission respectively, and $A$ represents the complex amplitude of the incident wave. Additionally, the reflectivity is given by the ratio,
\begin{equation}
  r = \frac{|R|^{2}}{|A|^{2}}
  \label{eqn:reflectivity}
\end{equation}

The refractive index of a medium can be expressed via Maxwell's formula,
\begin{equation*}
  n = \sqrt{\epsilon\mu}
\end{equation*}
where we can assume the magnetic permeability of ocean water is unity, such that
\begin{equation}
  n_{2} = \sqrt{\epsilon}
  \label{eqn:maxwells}
\end{equation}
Setting the refractive index of air to a value of 1.0, we can use equation \ref{eqn:maxwells} in Snell's law to obtain a substitution for $\cos\theta_{t}$,
\begin{eqnarray}
  \sqrt{\epsilon}\,\sin\theta_{t}  &=& \sin\theta_{i}\nonumber\\
  \textrm{i.e. }\sin^{2}\theta_{t} &=& \frac{\sin^{2}\theta_{i}}{\epsilon}\nonumber\\
  \cos^{2}\theta_{t}               &=& 1 - \frac{1 - \cos^{2}\theta_{i}}{\epsilon}\nonumber\\
                                   &=& \frac{\epsilon - 1 + \cos^{2}\theta_{i}}{\epsilon}\nonumber\\
  \therefore\:\cos\theta_{t}       &=& \sqrt{\frac{\epsilon - 1 + \cos^{2}\theta_{i}}{\epsilon}}
  \label{eqn:cost_substitution}
\end{eqnarray}
Substituting equations \ref{eqn:maxwells} and \ref{eqn:cost_substitution} into equation \ref{eqn:Rv_amplitude} and multiplying by $\sqrt{\epsilon}/\sqrt{\epsilon}$ we get,
\begin{eqnarray}
  R_{\parallel} &=& \frac{\sqrt{\epsilon}\,\cos\theta_{i} - \sqrt{\displaystyle\frac{\epsilon - 1 + \cos^{2}\theta_{i}}{\epsilon}}}{\sqrt{\epsilon}\,\cos\theta_{i} + \sqrt{\displaystyle\frac{\epsilon - 1 + \cos^{2}\theta_{i}}{\epsilon}}}.\frac{\sqrt{\epsilon}}{\sqrt{\epsilon}}.A_{\parallel}\nonumber\\\nonumber\\
                &=& \frac{\epsilon\,\cos\theta_{i} - \sqrt{\epsilon - 1 + \cos^{2}\theta_{i}}}{\epsilon\,\cos\theta_{i} + \sqrt{\epsilon - 1 + \cos^{2}\theta_{i}}}.A_{\parallel}
  \label{eqn:Rv_amplitude2}
\end{eqnarray}
with the reflectivity given by equation \ref{eqn:reflectivity}
\begin{equation}
  r_{\parallel} = \left|\frac{\epsilon\,\cos\theta_{i} - \sqrt{\epsilon - 1 + \cos^{2}\theta_{i}}}{\epsilon\,\cos\theta_{i} + \sqrt{\epsilon - 1 + \cos^{2}\theta_{i}}}\right|^{2}
  \label{eqn:Rv_reflectivity}
\end{equation}
Similarly for the equation \ref{eqn:Rh_amplitude},
\begin{eqnarray}
  R_{\perp} &=& \frac{\cos\theta_{i} - \sqrt{\epsilon}\,\sqrt{\displaystyle\frac{\epsilon - 1 + \cos^{2}\theta_{i}}{\epsilon}}}{\cos\theta_{i} + \sqrt{\epsilon}\,\sqrt{\displaystyle\frac{\epsilon - 1 + \cos^{2}\theta_{i}}{\epsilon}}}.A_{\perp}\nonumber\\\nonumber\\
                &=& \frac{\cos\theta_{i} - \sqrt{\epsilon - 1 + \cos^{2}\theta_{i}}}{\cos\theta_{i} + \sqrt{\epsilon - 1 + \cos^{2}\theta_{i}}}.A_{\perp}
  \label{eqn:Rh_amplitude2}
\end{eqnarray}
with reflectivity,
\begin{equation}
  r_{\perp} = \left|\frac{\cos\theta_{i} - \sqrt{\epsilon - 1 + \cos^{2}\theta_{i}}}{\cos\theta_{i} + \sqrt{\epsilon - 1 + \cos^{2}\theta_{i}}}\right|^{2}
  \label{eqn:Rh_reflectivity}
\end{equation}

